make freeze use the correct versions of add_get_carry and zselect

src/Arithmetic/Core.v
@@ -248,6 +248,7 @@ Require Import Crypto.Algebra.Nsatz.
 Require Import Crypto.Util.Decidable Crypto.Util.LetIn.
 Require Import Crypto.Util.ZUtil Crypto.Util.ListUtil Crypto.Util.Sigma.
 Require Import Crypto.Util.CPSUtil Crypto.Util.Prod.
+Require Import Crypto.Util.ZUtil.Zselect.
 Require Import Crypto.Arithmetic.PrimeFieldTheorems.
 Require Import Crypto.Util.Tactics.BreakMatch.
 Require Import Crypto.Util.Tactics.UniquePose.
@@ -833,39 +834,43 @@ Module B.
     End EvalHelpers.
 
     Section Select.
-      Context {weight : nat -> Z}
-              {select_single : Z -> Z -> Z}
-              {select_single_correct : forall cond x,
-                  select_single cond x = if dec (cond = 0) then 0 else x}
-      .
+      Context {weight : nat -> Z}.
       
-      Definition select_cps {n} cond (p : tuple Z n) {T} (f:_->T) :=
-        Tuple.map_cps (select_single cond) p f.
+      Definition select_cps {n} (mask cond:Z) (p:tuple Z n)
+                 {T} (f:tuple Z n->T) :=
+        dlet t := Z.zselect cond 0 mask in Tuple.map_cps (runtime_and t) p f.
 
-      Definition select {n} cond p := @select_cps n cond p _ id.
-      Lemma select_id {n} cond p T f :
-        @select_cps n cond p T f = f (select cond p).
+      Definition select {n} mask cond p := @select_cps n mask cond p _ id.
+      Lemma select_id {n} mask cond p T f :
+        @select_cps n mask cond p T f = f (select mask cond p).
       Proof.
-        cbv [select_cps select]. autorewrite with uncps push_id.
-        reflexivity.
+        cbv [select select_cps Let_In]; autorewrite with uncps push_id;
+          reflexivity.
       Qed.
       Hint Opaque select : uncps.
-      Hint Rewrite @select_id : uncps.
 
-      Lemma eval_select {n} cond p :
-        eval weight (@select n cond p) = if dec (cond = 0) then 0 else eval weight p.
+      Lemma map_and_0 {n} (p:tuple Z n) : Tuple.map (Z.land 0) p = zeros n.
       Proof.
-        cbv [select select_cps]; autorewrite with uncps push_id.
-        induction n; [destruct p|].
-        { break_match; reflexivity. }
-        { rewrite (Tuple.subst_left_append p).
-          rewrite Tuple.map_left_append, !eval_left_append.
-          rewrite select_single_correct, IHn.
-          break_match;  ring. }
-      Qed. Hint Rewrite @eval_select : push_basesystem_eval.
+        induction n; [destruct p; reflexivity | ].
+        rewrite (Tuple.subst_append p), Tuple.map_append, Z.land_0_l, IHn.
+        reflexivity.
+      Qed.
+
+      Lemma eval_select {n} mask cond x (H:Tuple.map (Z.land mask) x = x) :
+        B.Positional.eval weight (@select n mask cond x) =
+        if dec (cond = 0) then 0 else  B.Positional.eval weight x.
+      Proof.
+        cbv [select select_cps Let_In].
+        autorewrite with uncps push_id.
+        rewrite Z.zselect_correct; break_match.
+        { rewrite map_and_0. apply B.Positional.eval_zeros. }
+        {  change runtime_and with Z.land. rewrite H; reflexivity. }
+      Qed.
+
     End Select.
 
   End Positional.
+
   Hint Unfold
       Positional.add_cps
       Positional.mul_cps
@@ -941,33 +946,6 @@ Section DivMod.
     pose proof (Z.div_mod a b H). congruence.
   Qed.
 End DivMod.
-
-Section ZSelect.
-
-  Definition mask width cond :=
-    if dec (cond = 0) then 0 else Z.ones width.
-
-  Definition zselect bitwidth (cond x : Z) : Z :=
-    if (dec (x <= 0))
-    then (if dec (cond = 0) then 0 else x)
-    else (let width := Z.max (Z.log2 x + 1) bitwidth in
-          dlet t := mask width cond in x &' t).
-
-  Lemma zselect_correct bw cond x :
-    zselect bw cond x = if dec (cond = 0) then 0 else x.
-  Proof.
-    cbv [zselect mask Let_In]; break_match;
-      rewrite ?Z.land_0_r; try reflexivity; [ ].
-    pose proof (Z.log2_nonneg x).
-    pose proof (Z.log2_spec x) as Hlog2.
-    rewrite <-Z.add_1_r in Hlog2.
-    apply Z.max_case_strong; intros; rewrite Z.land_ones by omega;
-      apply Z.mod_small; split; try omega.
-    apply Z.lt_le_trans with (m:=2 ^ (Z.log2 x + 1));
-      [|apply Z.pow_le_mono_r]; omega.
-  Qed.
-
-End ZSelect.
 
 Import B.
 
